lib/basics.v
@@ -1,9 +1,11 @@
 Require Import String.
 Require Import Bool.
 Require Import List.
+Require Import Maps.
 From AC Require Import syntax.
 From AC Require Import nvalues.
-
+Require Import Coq.Program.Basics.
+Require Import Recdef.
 
 (*Not recursive on nvalues*)
 Reserved Notation "'/' x ':=' s '/' t" (in custom acnotation at level 20, x constr).
@@ -27,22 +29,24 @@ Fixpoint subst (x : string) (s : exp) (t : exp) : exp :=
 end
 where "'/' x ':=' s '/' t" := (subst x s t) (in custom acnotation).
 
+Require Import Psatz.
+Remark helper: forall t, 0 < exp_measure t.
+Proof.
+  induction t; compute; intuition.
+  destruct n.  destruct m. lia.
+Qed.
 
 (*Recursive on nvalues*)
-Fixpoint bounded (e:exp) (l_bounded:list string) {struct e}: Prop :=
-let l_b := 
-  (fix l_b (l : literal) : Prop := 
+Fixpoint bounded (e:exp) (l_bounded:list string)  {struct e}: Prop :=
+let fix l_b (l : literal) := 
         match l with
         | l_builtin b => True
-        | <{fun n [y:T] {t1}}> => 
-              bounded t1 (cons y l_bounded)
         | l_sensor s => True
         | l_fail => True
         | l_true => True
         | l_false => True
         | l_const n => True
         end
-    )
 in
 match e with 
   | exp_var y =>
@@ -54,11 +58,10 @@ match e with
   | <{fun n [y:T] {t1}}> =>
     bounded t1 (cons y l_bounded)
   | exp_nvalue w =>
-    (fix w_rec (w : nvalue ) : Prop := 
-    match w with
-      | default l => l_b l
-      | device _ l wl => l_b l /\ w_rec wl
-    end) w
+       match w with
+         (* TODO: use ∘, requires scope? *)
+       | nv (l, t) => let xs := (map snd (PTree.elements t)) in l_b l /\ forall x, In x xs -> l_b x
+       end
   | exp_literal l => l_b l
 end.
 
@@ -70,7 +73,7 @@ Inductive w_values : nvalue -> Prop :=
 
 Definition value (l:literal) : Prop := bounded (exp_literal l) nil.
 
-Definition w_value (w:nvalue):= ordered w /\ bounded (exp_nvalue w) nil.
+Definition w_value (w:nvalue):= bounded (exp_nvalue w) nil.
 
 Inductive is_fun: exp -> Prop :=
   | func : forall n x T2 t1, 
