lib/nvalues.v
@@ -1,49 +1,64 @@
 Require Import PeanoNat.
 From AC Require Import syntax.
 Require Import List.
+Require Import Maps.
+Require Import Ascii.
+Require Import BinPosDef.
+Require Import String.
+Require Import Pnat.
+
+Local Definition bool_cons_pos (b : bool) (p : positive) : positive :=
+  if b then p~1 else p~0.
+Local Definition ascii_cons_pos (c : ascii) (p : positive) : positive :=
+  match c with
+  | Ascii b0 b1 b2 b3 b4 b5 b6 b7 =>
+     bool_cons_pos b0 ( bool_cons_pos b1 ( bool_cons_pos b2 (
+       bool_cons_pos b3 ( bool_cons_pos b4 ( bool_cons_pos b5 (
+       bool_cons_pos b6 ( bool_cons_pos b7 p)))))))
+  end.
+Fixpoint string_to_pos (s : string) : positive :=
+  match s with
+  | EmptyString => 1
+  | String c s => ascii_cons_pos c (string_to_pos s)
+  end.
 
 (*get single device value*)
 Fixpoint get (pos:ident) (n:nvalue): literal :=
 match n with
-| default  x => x
-| device i x m => if (pos=?i) then x else (get pos m)
+| nv m => PMap.get (Pos.of_nat pos) m
 end.
 
 Fixpoint getDefault (n:nvalue): literal :=
 match n with
-| default x => x
-| device i x m => getDefault m
+| nv (x, _) => x
 end.
-
-(*ordered predicate*)
-Inductive ordered :nvalue -> Prop :=
-| ordered0 : forall x, ordered (default x)
-| ordered1 : forall a0 b0 b1, ordered ((device a0 b0 (default b1)))
-| ordered2 : forall a0 a1 m b0 b1, lt a0 a1 -> ordered (device a1 b1 m) -> ordered ((device a0 b0 (device a1 b1 m))).
 
 
 Fixpoint pointWise (op:literal -> literal -> literal) (w0:nvalue) {struct w0}: nvalue -> nvalue:=
-fix pointWise1 (w1:nvalue) {struct w1}: nvalue :=
-match w0,w1 with
-| default x , default y => default (op x y)
-| default x , device a b m  =>  device a (op x b) (pointWise1 m) 
-| device a b m , default x  => device a (op x b) (pointWise op  m (default x)) 
-| device a0 b0 m0 , device a1 b1 m1  => if (a0=?a1) then device a0 (op b0 b1) (pointWise op m0 m1)
-                                            else (if (a0<?a1) then device a0 (op b0 (getDefault m1)) (pointWise op m0 (device a1 b1 m1))
-                                            else device a1 (op (getDefault m0) b1) (pointWise1 m1 ))
-end.
+  fix pointWise1 (w1:nvalue) {struct w1}: nvalue :=
+    match w0,w1 with
+    | nv (e1,t1), nv (e2,t2) => nv (op e1 e2, PTree.combine
+                                                (fun x y => match x,y with
+                                                            | None, None => None
+                                                            | None, Some z => Some z
+                                                            | Some z, None => Some z
+                                                            | Some zx, Some zy => Some (op zx zy)
+                                                            end)
+                                                t1 t2)
+    end.
 
 Fixpoint extend (w0:nvalue) {struct w0}: nvalue -> nvalue:=
-fix extend1 (w1:nvalue) {struct w1}: nvalue :=
-match w0,w1 with
-| default x , default y => default x
-| default x , device a b m  =>  device a x (extend1 m) 
-| device a b m , default x  => device a b (extend m w1)
-| device a0 b0 m0 , device a1 b1 m1  => if (a0=?a1) then device a0 b0 (extend m0 m1)
-                                            else (if (a0<?a1) then device a0 b0 (extend m0 w1)
-                                            else device a1 (getDefault w0) (extend1 m1))
-end. 
-
+  fix extend1 (w1:nvalue) {struct w1}: nvalue :=
+    match w0,w1 with
+    | nv (e1,t1), nv (e2,t2) => nv (e1 (*!*), PTree.combine
+                                                (fun x y => match x,y with
+                                                            | None, None => None
+                                                            | None, Some z => Some z
+                                                            | Some z, None => Some z
+                                                            | Some zx, Some zy => Some zx
+                                                            end)
+                                                t1 t2)
+    end.
 
 
 Fixpoint folding (delta:ident) (devs:list nat) (w1:nvalue) (w2:nvalue) (w3:nvalue) : exp :=
@@ -51,5 +66,4 @@ match devs with
 | cons id l => if (delta =? id) then (folding id l w1 w2 w3) else exp_app (exp_app w1 (nvalues.get id w2)) (folding delta l w1 w2 w3)
 | nil => (get delta w3)
 end.
-
 
