lib/sensor_state.v
@@ -1,24 +1,25 @@
 From AC Require Import syntax.
+From AC Require Import nvalues.
 Require Import String.
 Require Import Bool.
 Require Import Coqlib.
 Require Import Maps.
-Require Import Coq.Strings.BinaryString.
 
 Set Implicit Arguments.
 
 (* Have: *)
 Definition sensor_state := PMap.t nvalue.
 
-Definition getSens (n:string) (s:sensor_state) : nvalue := PMap.get (to_pos n) s.
+Definition getSens (n:string) (s:sensor_state) := PMap.get (string_to_pos n) s.
+
 
 (* END *)
-Definition base (s:string) := default l_fail.
+Definition base (s:string) : sensor_state := PMap.init (nv (PMap.init l_fail)).
 
-Definition contains (s:string) (old:sensor_state): bool := 
-match (PMap.get (to_pos s) old) with 
-| default l_fail => false
-| _ => true
+(*Definition contains (s:string) (old:sensor_state): bool := 
+match (PMap.get (string_to_pos s) old) with 
+| nv (_,t) => PTree.empty t
 end.
+ *)
 
-Definition add (s:string) (v:nvalue) (old:sensor_state): sensor_state := PMap.set (to_pos s) v old.
+Definition add (s:string) (v:nvalue) (old:sensor_state): sensor_state := PMap.set (string_to_pos s) v old.
