lib/value_tree.v
@@ -3,6 +3,8 @@ Require Import String.
 Require Import PeanoNat. 
 Require Import List. 
 Require Import nvalues.
+Require Import Maps.
+Require Import Coq.PArith.BinPosDef.
 
 Inductive value_tree: Type :=
 | empty : list value_tree -> value_tree
@@ -10,7 +12,7 @@ Inductive value_tree: Type :=
 
 Definition rho (v:value_tree) : nvalue :=
 match v with 
-| empty _ => default l_fail
+| empty _ => nv (PMap.init l_fail)
 | some w _ => w
 end.
 
@@ -65,22 +67,17 @@ end.
 
 Fixpoint get_messages (my_id:ident) (w_i:nvalue) (v_env:value_tree_env) : nvalue :=
 match v_env with
-| vt_el id vt v_env_next => device id (nvalues.get my_id (rho vt)) (get_messages my_id w_i v_env_next) 
-| v_end => default (nvalues.getDefault w_i) (*nvalue dentro nvalue ?*)
+| vt_el id vt v_env_next => nv (PMap.set (Pos.of_nat id) (nvalues.get my_id (rho vt)) ((fun nvm => match nvm with | nv m => m end) (get_messages my_id w_i v_env_next)))
+| v_end => nv (PMap.init (nvalues.getDefault w_i) (*nvalue dentro nvalue ?*))
 end.
 (* Se dentro a un nvalue di un value_tree non è presente 
 il valore per il nostro dispositivo è sufficiente il default? *)
 
-
+(*
 Compute (get_messages 2 <{[>5]}> (vt_el 3 (some <{[2>>5][>6]}> nil) 
 (vt_el 4 (some <{[1>>2][2>>6][>7]}> nil) (vt_el 7 (some <{[1>>2][2>>6][>7]}> nil) vt_end ) )  )).
 
 Compute (get_messages 2 <{[>5]}> (vt_el 3 (some <{[2>>5][>6]}> nil) 
 (vt_el 4 (some <{[1>>2][2>>6][>7]}> nil) (vt_el 7 (empty nil) vt_end ) )  )).
 
-
-
-
-
-
-
+*)
